theories/Compositional_Structures/Basic_Modules/Component_Types/Social_Choice_Types/Profile_Sepref.thy
@@ -11,7 +11,7 @@ definition "ballot_rel A \<equiv> br pl_\<alpha> (ballot_on A)"
 
 definition "ballot_assn A \<equiv> hr_comp (array_assn id_assn) (ballot_rel A)"
 
-abbreviation "cand_assn \<equiv> (id_assn::(nat) \<Rightarrow> _)"
+(*abbreviation "cand_assn \<equiv> (id_assn::(nat) \<Rightarrow> _)"*)
 
 
 sepref_definition idx_imp is 
@@ -34,7 +34,7 @@ lemmas idx_imp_correct = idx_imp.refine[FCOMP index_mon_refine]
 
 sepref_definition rank_imp is
   "uncurry rank_mon" :: "(array_assn nat_assn)\<^sup>k *\<^sub>a (nat_assn)\<^sup>k \<rightarrow>\<^sub>a nat_assn"
-  unfolding rank_mon_def[abs_def] index_mon_def[abs_def] index_mon_inv_def[abs_def]
+  unfolding rank_mon_def[abs_def] index_mon_def[abs_def]
   by sepref
 
 lemmas rank_imp_correct = rank_imp.refine[FCOMP rank_mon_refine]
@@ -42,18 +42,19 @@ lemmas rank_imp_correct = rank_imp.refine[FCOMP rank_mon_refine]
 
 definition "profile_rel A \<equiv> br pl_to_pr_\<alpha> (profile_l A)"
 
-abbreviation "profile_impl_assn \<equiv> array_assn (array_assn nat_assn)"
+(*abbreviation "profile_impl_assn \<equiv> array_assn (array_assn nat_assn)"
 
 definition "profile_assn A
-    \<equiv> hr_comp profile_impl_assn (profile_rel A)"
+    \<equiv> hr_comp profile_impl_assn (profile_rel A)"*)
 
 sepref_definition win_count_imp_sep is
-  "uncurry win_count_imp" :: "(profile_impl_assn)\<^sup>k *\<^sub>a (nat_assn)\<^sup>k \<rightarrow>\<^sub>a nat_assn"
-  unfolding win_count_imp_def[abs_def] 
-    rank_mon_def[abs_def]
-  apply sepref_dbg_keep
-      apply sepref_dbg_trans_keep
- apply sepref_dbg_trans_step_keep
+  "uncurry win_count_list_r_mon" :: "(array_assn (array_assn nat_assn))\<^sup>k *\<^sub>a (nat_assn)\<^sup>k \<rightarrow>\<^sub>a nat_assn"
+  unfolding win_count_list_r_mon_def[abs_def] rank_mon_def[abs_def] index_mon_def[abs_def] 
+    using rank_mon_correct index_mon_correct
+  apply (sepref_dbg_keep)
+       apply sepref_dbg_constraints
+      apply sepref_dbg_trans_step_keep
+    oops
 
 
 end
